Maxwell's equations, as ordinarily written, are (\footnote{Equations (\ref{ecuacion 22.3}) and (\ref{ecuacion 
22.4}) are logical consequences of (\ref{ecuacion 22.1}) and (\ref{ecuacion 22.2}). As a consequence they can be 
omitted.}):
\begin{equation}
 \label{ecuacion 23.1}
 E = - \frac{1}{c}\frac{\partial A}{\partial t} - \mbox{grad }\phi,
\end{equation}
\begin{equation}
 \label{ecuacion 23.2}
 H = \mbox{curl } A,
\end{equation}
\begin{equation}
 \label{ecuacion 23.3}
 \frac{1}{c}\frac{\partial H}{\partial t} = - \mbox{curl } E,
\end{equation}
\begin{equation}
 \label{ecuacion 23.4}
 \mbox{div } H = 0,
\end{equation}
\begin{equation}
 \label{ecuacion 23.5}
 \frac{1}{c}\frac{\partial E}{\partial t} = \mbox{curl } H - 4 \pi j,
\end{equation}
\begin{equation}
 \label{ecuacion 23.6}
 \mbox{div } E = 4 \pi \rho.
\end{equation}






