Let us consider a static gravitational field and refer it to a static coordinate system. The $g_{\mu\nu}$ are then 
constant in time, $g_{\mu\nu,0} = 0$. Further, we must have 
\[
 g_{m0} = 0, \, \left( m=1,\cdots,3 \right) .
\]
This leads to
\[
 g^{m0} = 0, \, g^{00} = (g_{00})^{-1},
\]
and $g^{mn}$ is the reciprocal matrix to $g_{mn}$. Roman suffixes like $m$ and $n$ always take on the values 1, 2, 3. 
We find that $\Gamma_{m0n} = 0$ and hence also $\Gamma^{m}_{0n}=0$.

Let us take a particle that is moving slowly, compared with the velocity of light. Then $v^m$ is a small quantity, of 
the first order. With neglect of second order quantities,
\begin{equation}
 \label{ecuacion 16.1}
 g_{00} {v^{0}}^2 = 1.
\end{equation}

The particle will move along a geodesic. With neglect of second-order quantities, equation (\ref{ecuacion 8.3}) gives
\[
 \begin{array}{rcl}
  \frac{dv^m}{ds} & = & -\Gamma^m_{00} {v^0}^2 = - g^{mn}\Gamma_{n00} {v^0}^2 \\
  & = & \frac{1}{2} g^{mn} \Gamma_{n00} {v^0}^2 .
 \end{array}
\]
Now
\[
 \frac{dv^m}{d s} = \frac{d v^m}{dx^0} \frac{d x^0}{ds} = \frac{d v^m}{dx^0} \frac{d x^0}{ds}
\]
to the first order. Thus
\begin{equation}
 \label{ecuacion 16.2}
 \frac{dv^m}{dx^0} = \frac{1}{2} g^{mn} g_{00,n} v^0 = g^{mn}\left( g_{00}\right)^{1/2}_{,n}
\end{equation}
with the help of (\ref{ecuacion 16.1})(\footnote{Because ${v^0} = 
\frac{1}{\sqrt{g_00}}$}.) Notice that here we are taking the positive square root. Since the $g_{\mu\nu}$ are 
independent of $x^0$, we may lower the suffix $m$ here and get
\begin{equation}
 \label{ecuacion 16.3}
 \frac{dv_m}{dx^0} = \left( g_{00} \right)^{1/2}_{,m}.
\end{equation}

We see that the particle moves as if it were under the influence of a potential $\left( g_{00} \right)^{1/2}$. We have 
not used Einstein's law to obtain this result. We now use Einstein's law to obtain a condition for the potential, so 
that it can be compared with Newton's.









